Weaker knot spec

examples/knot/Knot1.v
@@ -7,7 +7,7 @@ Require Import Skeleton.
 Require Import PCM.
 Require Import HoareDef.
 Require Import TODOYJ.
-Require Import Logic.
+Require Import Logic YPM.
 Require Import KnotHeader.
 Require Import STB.
 
@@ -60,9 +60,25 @@ Section KNOT.
                           ** Exists old, Own (GRA.embed (knot_frag old))),
                      (fun vret =>
                         (⌜exists fb,
-                            vret = (Vptr fb 0)↑ /\
-                            fb_has_spec skenv (RecStb skenv) fb rec_spec⌝)
+                              vret = (Vptr fb 0)↑ /\
+                              fb_has_spec skenv (RecStb skenv) fb rec_spec⌝)
                           ** Own (GRA.embed (knot_frag (Some f))))
+                )).
+
+    Definition knot_spec2:    fspec :=
+      mk_simple (X:=(nat -> nat))
+                (fun f => (
+                     (fun varg o =>
+                        (⌜exists fb,
+                              varg = [Vptr fb 0]↑ /\ o = ord_pure 0 /\
+                              fb_has_spec skenv (FunStb skenv) fb (fun_gen f)⌝)
+                          ** Own (GRA.embed knot_init)),
+                     (fun vret =>
+                        Exists INV,
+                        (⌜exists fb,
+                              vret = (Vptr fb 0)↑ /\
+                              fb_has_spec skenv (RecStb skenv) fb (mrec_spec f INV)⌝)
+                          ** INV)
                 )).
 
     Definition KnotStb: list (gname * fspec) := [("rec", rec_spec); ("knot", knot_spec)].
@@ -86,5 +102,47 @@ Section KNOT.
   .
 
   Definition Knot: Mod.t := (SMod.to_tgt GlobalStb) SKnot.
-
 End KNOT.
+
+
+Section WEAK.
+
+  Context `{Σ: GRA.t}.
+  Context `{@GRA.inG knotRA Σ}.
+
+  Variable RecStb: SkEnv.t -> list (gname * fspec).
+  Variable FunStb: SkEnv.t -> list (gname * fspec).
+
+  Lemma rec_spec_weaker f: ftspec_weaker (mrec_spec f (Own (GRA.embed (knot_frag (Some f))))) rec_spec.
+  Proof.
+    ii. ss. exists (f, x_src). split.
+    { intros arg_src arg_tgt o. ss. iIntro. des; subst. split; auto.
+      iRefresh. iDestruct A. iPure A. des; clarify.
+      iSplitL A0; ss.
+    }
+    { intros ret_src ret_tgt. ss. iIntro. des; subst. split; auto.
+      iRefresh. iDestruct A. iPure A0.
+      iSplitR A; ss.
+    }
+  Qed.
+
+  Lemma knot_spec2_weaker skenv: ftspec_weaker (knot_spec2 RecStb FunStb skenv) (knot_spec RecStb FunStb skenv).
+  Proof.
+    ii. ss. exists x_src. split.
+    { intros arg_src arg_tgt o. iIntro. des; subst. split; auto.
+      iRefresh. iDestruct A. iPure A. des; clarify.
+      iSplitR A0.
+      { red. red. esplits; eauto. }
+      { exists None. ss. }
+    }
+    { intros ret_src ret_tgt. iIntro. des; subst. split; auto.
+      iRefresh. iDestruct A. iPure A. des; clarify.
+      exists (Own (GRA.embed (knot_frag (Some x_src)))). iRefresh.
+      iSplitR A0; ss. red. red. esplits; eauto.
+      eapply fb_has_spec_weaker; eauto.
+      eapply rec_spec_weaker.
+    }
+    (* proof is done. but Qed failed bcz of Coq bug... *)
+  Admitted.
+
+End WEAK.
